theories/Util/Iteration.v
@@ -45,4 +45,48 @@ Section iteration.
         end
     end.
 
+  Fixpoint filter_map (ls : list T) : list U :=
+    match ls with
+      | nil => nil
+      | l :: ls => match f l with
+                     | None => filter_map ls
+                     | Some x => x :: filter_map ls
+                   end
+    end.
+
+  Lemma filter_map_sound
+  : forall ls,
+      Forall (fun x => exists l, In l ls /\ f l = Some x)
+             (filter_map ls).
+  Proof.
+    clear. induction ls; simpl; intros.
+    { constructor. }
+    { assert (Forall (fun x : U => exists l : T, (a = l \/ In l ls) /\ f l = Some x)
+                     (filter_map ls)).
+      { eapply Forall_impl; eauto.
+        simpl in *. intuition.
+        destruct H as [ ? [ ? ? ] ].
+        eexists; split. right. eassumption. eauto. }
+      { consider (f a); intros; auto.
+        constructor; eauto. } }
+  Qed.
+
+  Lemma in_filter_map_iff : forall ls x,
+                              List.In x (filter_map ls) <->
+                              exists y, f y = Some x /\ List.In y ls.
+  Proof.
+    clear.
+    induction ls; simpl.
+    { intuition. destruct H; intuition. }
+    { intuition.
+      { consider (f a); intros.
+        { destruct H0. subst. eauto.
+          eapply IHls in H0. destruct H0. intuition; eauto. }
+        { eapply IHls in H0. destruct H0; intuition; eauto. } }
+      { destruct H. destruct H.
+        destruct H0; subst.
+        { rewrite H. left. auto. }
+        { destruct (f a); try right; apply IHls; eauto. } } }
+  Qed.
+
 End iteration.
